convert/graph.py
@@ -6,7 +6,6 @@ import json
 from typing import Tuple, List, Set, Dict, Any, AnyStr, Optional, Union
 # from connected_components import *
 from treeSet import Tree
-from treeMap import Map
 
 class Edge():
     fst : int
