src/hog/Graph.lean
@@ -39,7 +39,6 @@ instance Graph_edge_Fintype (G : Graph) : Fintype G.edge := by
 def Graph.edgeSize (G : Graph) := Fintype.card G.edge
 
 -- the vertex adjacency relation
-@[simp]
 def Graph.badjacent {G : Graph} : G.vertex → G.vertex → Bool :=
   fun u v =>
     lt_by_cases u v
@@ -47,54 +46,52 @@ def Graph.badjacent {G : Graph} : G.vertex → G.vertex → Bool :=
       (fun _ => false)
       (fun v_lt_u => G.edgeTree.mem (Edge.mk u (Fin.mk v v_lt_u)))
 
-@[simp]
 def Graph.adjacent {G : Graph} : G.vertex → G.vertex → Prop :=
   fun u v => G.badjacent u v
 
 -- adjacent vertices induce an edge
-@[simp]
 def Graph.adjacentEdge {G : Graph} {u v : G.vertex} :
   G.adjacent u v → G.edge := by
   apply lt_by_cases u v
   · intros u_lt_v uv
     constructor
     case val => exact Edge.mk v ⟨u, u_lt_v⟩
-    case property => simp_all [u_lt_v, lt_by_cases]
+    case property => simp_all [u_lt_v, lt_by_cases, adjacent, badjacent]
   · intro u_eq_v
     intro H
-    simp [u_eq_v, lt_by_cases] at H
+    simp [u_eq_v, lt_by_cases, adjacent, badjacent] at H
   · intros v_lt_u uv
     constructor
     case val => exact Edge.mk u ⟨v, v_lt_u⟩
-    case property => simp_all [v_lt_u, not_lt_of_lt, lt_by_cases]
+    case property => simp_all [v_lt_u, not_lt_of_lt, lt_by_cases, adjacent, badjacent]
 
 lemma Graph.adjacentEdge_lt_fst {G : Graph} {u v : G.vertex} (uv : G.adjacent u v):
   u < v -> G.fst (G.adjacentEdge uv).val = v := by
   intro u_lt_v
-  simp [u_lt_v, lt_by_cases]
+  simp [u_lt_v, lt_by_cases, adjacentEdge]
 
 lemma Graph.adjacentEdge_gt_fst {G : Graph} {u v : G.vertex} (uv : G.adjacent u v):
   v < u -> G.fst (G.adjacentEdge uv).val = u := by
   intro v_lt_u
-  simp [v_lt_u, not_lt_of_lt, lt_by_cases]
+  simp [v_lt_u, not_lt_of_lt, lt_by_cases, adjacentEdge]
 
 lemma Graph.adjacentEdge_lt_snd {G : Graph} {u v : G.vertex} (uv : G.adjacent u v):
   u < v -> G.snd (G.adjacentEdge uv).val = u := by
   intro u_lt_v
   apply Fin.eq_of_val_eq
-  simp [u_lt_v, lt_by_cases]
-  sorry
-
+  simp [Fin.eq_of_val_eq, adjacentEdge, lt_by_cases, u_lt_v, not_lt_of_lt]
+  sorry 
+  
 lemma Graph.adjacentEdge_gt_snd {G : Graph} {u v : G.vertex} (uv : G.adjacent u v):
   v < u -> G.snd (G.adjacentEdge uv).val = v := by
   sorry
 
 lemma Graph.irreflexiveNeighbor (G : Graph) :
-  ∀ (v : G.vertex), ¬ adjacent v v := by simp [lt_by_cases]
+  ∀ (v : G.vertex), ¬ adjacent v v := by simp [lt_by_cases, adjacent, badjacent]
 
 lemma Graph.symmetricNeighbor (G : Graph) :
   ∀ (u v : G.vertex), adjacent u v → adjacent v u := by
     intros u v
-    apply lt_by_cases u v <;> (intro h ; simp [lt_by_cases, not_lt_of_lt, h])
+    apply lt_by_cases u v <;> (intro h ; simp [lt_by_cases, not_lt_of_lt, h, adjacent, badjacent])
 
 end HoG
