src/hog/JsonDecoder.lean
@@ -1,6 +1,8 @@
 import Qq
 import Graph
 import EdgeSize
+import ConnectedComponents
+import TreeMap
 
 set_option autoImplicit false
 
@@ -16,13 +18,50 @@ def edgeOfJson (n : Q(Nat)) (j : Lean.Json) : Except String Q(Edge $n) := do
   have H2 : Q(Nat.blt $b $a = true) := (q(Eq.refl true) : Lean.Expr)
   pure q(Edge.mk' $n $a $b $H1 $H2)
 
+def natOfJson (j : Lean.Json) : Except String Q(Nat) := do
+  have n : Q(Nat) := Lean.mkRawNatLit (← j.getNat?)
+  pure n
+
+def finOfJson (n : Q(Nat)) (j : Lean.Json) : Except String Q(Fin $n) := do
+  have k : Q(Nat) := Lean.mkRawNatLit (← j.getNat?)
+  have H : Q(Nat.blt $k $n = true) := (q(Eq.refl true) : Lean.Expr)
+  pure q(Fin.mk $k (Nat.le_of_ble_eq_true $H))
+
+def vertexOfJson (G : Q(Graph)) (j : Lean.Json) : Except String Q(Graph.vertex $G) := do
+  finOfJson (q(Graph.vertexSize $G)) j
+
 partial def treeOfJson (n : Q(Nat)) (j : Lean.Json) : Except String Q(STree (Edge $n)) := do
   let arr ← j.getArr?
   match arr with
-  | #[e, l, r] => pure q(STree.node $(← edgeOfJson n e) $(← treeOfJson n l) $(← treeOfJson n r))
   | #[] => pure q(STree.empty)
   | #[v] => pure q(STree.leaf $(← edgeOfJson n v))
+  | #[e, l, r] => pure q(STree.node $(← edgeOfJson n e) $(← treeOfJson n l) $(← treeOfJson n r))
   | _ => throw "invalid tree format"
+
+partial def mapTreeOfJson (α β : Q(Type))
+  (keyOfJson : Lean.Json → Except String Q($α))
+  (valOfJson : Lean.Json → Except String Q($β))
+  (j : Lean.Json) : Except String Q(Map $α $β) := do
+  let arr ← j.getArr?
+  match arr with
+  | #[] => pure q(Map.empty)
+  | #[k, v] => pure q(Map.leaf $(← keyOfJson k) $(← valOfJson v))
+  | #[k, v, l, r] => pure q(Map.node $(← keyOfJson k) $(← valOfJson v) $(← mapTreeOfJson α β keyOfJson valOfJson l) $(← mapTreeOfJson α β keyOfJson valOfJson r))
+  | _ => throw "invalid tree map format"
+
+partial def mapOfJson (α β : Q(Type))
+  (keyOfJson : Lean.Json → Except String Q($α))
+  (valOfJson : Lean.Json → Except String Q($β))
+  (j : Lean.Json) : Except String Q($α → $β) := do
+  let arr ← j.getArr?
+  match arr with
+  | #[] => _ -- empty domain
+  | #[treeJ, defaultJ] =>
+    let tree ← mapTreeOfJson α β keyOfJson valOfJson treeJ
+    let defaultValue ← valOfJson defaultJ
+    pure q(Map.getD $tree $defaultValue) 
+  | _ => throw "invalid map format"
+
 
 partial def graphOfJson (j : Lean.Json) : Except String Q(Graph) := do
     let json_v ← j.getObjVal? "vertexSize"
@@ -31,48 +70,43 @@ partial def graphOfJson (j : Lean.Json) : Except String Q(Graph) := do
     pure q(Graph.mk $v $edges)
 
 def edgeSizeOfJson (G : Q(Graph)) (j : Lean.Json) : Except String Q(EdgeSize $G) := do
-  let j ← j.getObjVal? "edgeSize"
   have e : Q(Nat) := Lean.mkRawNatLit (← j.getNat?)
   have H : Q(Nat.beq ($G).edgeTree.size $e = true) := (q(Eq.refl true) : Lean.Expr)
   pure q(EdgeSize.mk' $G $e $H)
 
+def componentsCertificateOfJson (G : Q(Graph)) (j : Lean.Json) : Except String Q(ComponentsCertificate $G) := do
+  let valJ ← j.getObjVal? "val"
+  have val : Q(Nat) := Lean.mkRawNatLit (← valJ.getNat?)
+  let componentJ ← j.getObjVal? "component"
+  let componentMap ← mapOfJson q(Graph.vertex $G) q(Fin $val) (vertexOfJson G) (finOfJson val) componentJ
+  let rootJ ← j.getObjVal? "root"
+  let rootMap ← mapOfJson q(Graph.vertex $G) q(Graph.vertex $G) (vertexOfJson G) (vertexOfJson G) rootJ
+  let nextJ ← j.getObjVal? "next"
+  let nextMap ← mapOfJson q(Graph.vertex $G) q(Graph.vertex $G) (vertexOfJson G) (vertexOfJson G) nextJ
+  let distToRootJ ← j.getObjVal? "distToRoot"
+  let distToRootMap ← mapOfJson q(Graph.vertex $G) q(Graph.vertex $G) (vertexOfJson G) natOfJson distToRootJ
+  sorry -- we need a smart constructor here
+
 -- The Lean name generated from a string
 def hogName (hogId : String) : Lean.Name := (.str (.str .anonymous "HoG") hogId)
 
+-- A name for an instance of a particular HoG
 def hogInstanceName (hogId : String) (inst : String) : Lean.Name :=
   (.str (hogName hogId) inst)
-
--- loading a hog as a function
--- def loadHog (hogId : String) : IO Unit  := do
---   let packageDir ← Mathlib.getPackageDir "HoG"
---   let dataDir := ((packageDir.join "..").join "..").join "pigpen" -- folder with the JSON files
---   let fileName := (dataDir.join hogId).withExtension "json"
---   let file ← IO.FS.readFile fileName
---   let graph : Except String (Q(Graph)) := do
---     let json ← Lean.Json.parse file
---     graphOfJson json
---   let .ok value := graph | throw (IO.userError "could not load the JSON file")
---   whatToDoHere <| Lean.addAndCompile <| .defnDecl {
---     name := hogName hogId
---     levelParams := []
---     type := q(Graph)
---     value
---     hints := .regular 0
---     safety := .safe
---   }
 
 -- lifting from exception monad to the Elab.Command monad
 def liftExcept {α : Type} : Except String α → Lean.Elab.Command.CommandElabM α
   | .ok res => pure res
   | .error msg => throwError msg
 
-elab "loadHog" hogId:str : command => do
+elab "#loadHog" hogId:str : command => do
   let packageDir ← Mathlib.getPackageDir "HoG"
   let dataDir := ((packageDir.join "..").join "..").join "pigpen" -- folder with the JSON files
   let fileName := (dataDir.join hogId.getString).withExtension "json"
   let file ← IO.FS.readFile fileName
   let json ← liftExcept <| Lean.Json.parse file
-  let graphQ : Q(Graph) ← liftExcept <| graphOfJson json
+  let graphJ ← liftExcept <| json.getObjVal? "graph"
+  let graphQ : Q(Graph) ← liftExcept <| graphOfJson graphJ
   -- load the graph
   let graphName := hogName hogId.getString
   Lean.Elab.Command.liftCoreM <| Lean.addAndCompile <| .defnDecl {
@@ -86,7 +120,8 @@ elab "loadHog" hogId:str : command => do
   have graph : Q(Graph) := Lean.mkConst graphName []
   -- load the edgeSize instance
   let edgeSizeName := hogInstanceName hogId.getString "edgeSizeI"
-  let edgeSizeQ : Q(EdgeSize $graph) ← liftExcept <| edgeSizeOfJson graph json
+  let edgeSizeJ ← liftExcept <| json.getObjVal? "edgeSize"
+  let edgeSizeQ : Q(EdgeSize $graph) ← liftExcept <| edgeSizeOfJson graph edgeSizeJ
   Lean.Elab.Command.liftCoreM <| Lean.addAndCompile <| .defnDecl {
     name := edgeSizeName
     levelParams := []
@@ -96,9 +131,21 @@ elab "loadHog" hogId:str : command => do
     safety := .safe
   }
   Lean.Elab.Command.liftTermElabM <| Lean.Meta.addInstance edgeSizeName .scoped 42
+  -- load the components certificate
+  let componentsCertificateName := hogInstanceName hogId.getString "componentsCertificateI"
+  let componentsCertificateJ ← liftExcept <| json.getObjVal? "componentsCertificate"
+  let componentsCertificateQ : Q(ComponentsCertificate $graph) ← liftExcept <| componentsCertificateOfJson graph componentsCertificateJ
+  Lean.Elab.Command.liftCoreM <| Lean.addAndCompile <| .defnDecl {
+    name := componentsCertificateName
+    levelParams := []
+    type := q(ComponentsCertificate $graph)
+    value := componentsCertificateQ
+    hints := .regular 0
+    safety := .safe
+  }
 
-loadHog "hog00000"
-#eval (hog00000.edgeSizeI.val)
+#loadHog "hog00001"
+#eval (hog00001.edgeSizeI.val)
 
 
 -- elab "getHog" hogId:str : term => do
